

1. Observe that

4 marks {

$$\begin{aligned}
 P_{0X^{-1}}(A) &= P[\omega \in \Omega : X(\omega) \in A] \\
 &= P[\omega \in \Omega : X(\omega) \leq \ln 2] \\
 &= P[\omega \in \Omega : -\ln(1-\omega) \leq \ln 2] \\
 &= P[\omega \in \Omega : \ln\left(\frac{1}{1-\omega}\right) \leq \ln 2] \\
 &= P[\omega \in \Omega : \frac{1}{1-\omega} \leq 2] \text{ since } \ln \uparrow \\
 &= P[\omega \in \Omega : 1-\omega \leq \frac{1}{2}] \\
 &= P[\omega \in \Omega : \omega \geq \frac{1}{2}].
 \end{aligned}$$

2 marks {

Now, $\Omega = (0, 1)$, $IP((a, b)) = b - a$

so, $IP[\omega \in (0, 1) : \omega \in (\frac{1}{2}, 1)]$

$= 1 - \frac{1}{2} = \frac{1}{2}$. (Answer).

2. 3 marks {

X : RV. $M_X(t) = e^{\frac{t^2}{2}} \Rightarrow X \sim N(0, 1)$.

Now, $Y(\omega) = \Phi(X(\omega)) \forall \omega \in \Omega$, where

$$\Phi(x) = \frac{1}{\sqrt{2\pi}} \int_{-\infty}^x e^{-\frac{y^2}{2}} dy.$$

so, $Y \sim \text{Unif}(0, 1)$. [Proof is NOT required; taught in class].

3 marks {

Now, $\sum_{n=0}^{\infty} \{E[Y^n]\}^2 = \sum_{n=0}^{\infty} \frac{1}{(n+1)^2} < \infty$.

so, it is true.

3. Take ~~$k \in \mathbb{R}$~~
 Consider $p \in (0, k)$. & $Y(\omega) = \{X(\omega)\}^p \forall \omega \in \Omega$.
 ~~g~~ so, $\frac{k}{p} > 1$.
 Consider $g(Y) = Y^{\frac{k}{p}}$, where $g: (0, \infty) \rightarrow (0, \infty)$.
 Observe that $g(Y)$ is a convex
 $f^{\frac{k}{p}}$ (Proof is not required; proof is straight forward).

Therefore, by Jensen's inequality, we have

$g(E(Y)) \leq E g(Y)$.
 $\Rightarrow \{E Y\}^{\frac{k}{p}} \leq E(Y^{\frac{k}{p}})$
 $\Rightarrow \{E X^p\}^{\frac{k}{p}} \leq E(X^{p \times \frac{k}{p}}) = E X^k$
 $\Rightarrow \{E X^p\}^{\frac{1}{p}} \leq \{E X^k\}^{\frac{1}{k}}$ since $k \in [0, \infty)$.
 Since $p \in (0, k)$, the above implies
 and it is true for
 all $p \in (0, k)$
 that $(E X^k)^{\frac{1}{k}}$ is an increasing $f^{\frac{1}{k}}$ in $k \in [0, \infty)$.

4.

(i) Yes, X & Y are identically distributed

since $F_X(a) = F_Y(a) \forall a \in \mathbb{R}$, where

$F_X(\cdot)$ & $F_Y(\cdot)$ are the CDF of X & Y , respectively.

→ 1.5 marks (if it is NOT shown).

(ii) Since $F_X(a) = F_Y(a) \forall a \in \mathbb{R}$,

$$E(X^n) = E(Y^n) \forall n \in \mathbb{N}.$$

Answer: Yes.

Alternative argument:- Direct integration &

show that $E X^n = E Y^n \forall n \in \mathbb{N}$.

(iii) Since $F_X(a) = F_Y(a) \forall a \in \mathbb{R}$,

~~so it is enough to derive~~
 $E(X^{2m}) = E(Y^{2m}) \forall m \in \mathbb{N}.$

$$\text{Now, } E(Y^{2m}) = E(X^{2m})$$

$$= \frac{1}{\sqrt{2\pi}} \int_{-\infty}^{\infty} x^{2m} e^{-\frac{x^2}{2}} dx$$

After a

$$\text{few steps } = (2m-1)(2m-3) \times \dots \times 5 \times 3 \times 1.$$

Alternative argument:- Directly compute

$$E(Y^{2m}) = \int_{-\infty}^{\infty} y^{2m} (\dots) dy.$$

5. (i) Observe that

$$\begin{aligned}
 F_X(x) &= \int_{-\infty}^x f_X(y) dy = \begin{cases} 0 & \text{if } x < -1 \\ \int_{-1}^x f_X(y) dy & \text{if } -1 \leq x \leq 0 \\ \int_{-1}^0 f_X(y) dy + \int_0^x f_X(y) dy & \text{if } 0 < x \leq \frac{3}{2} \\ 1 & \text{if } x > \frac{3}{2} \end{cases} \\
 \downarrow \\
 \text{CDF of } X & \\
 &= \begin{cases} 0 & \text{if } x < -1 \\ \frac{x+1}{2} & \text{if } -1 \leq x \leq 0 \\ \frac{1}{2} + \frac{x}{3} & \text{if } 0 < x \leq \frac{3}{2} \\ 1 & \text{if } x > \frac{3}{2} \end{cases} \quad \text{--- (**) }
 \end{aligned}$$

Further, observe that

$$\begin{aligned}
 F_Y(y) &= P[X^4 \leq y] = P[-y^{\frac{1}{4}} \leq X \leq y^{\frac{1}{4}}] \\
 \downarrow \\
 \text{CDF of } Y & \\
 &= F_X(y^{\frac{1}{4}}) - F_X(-y^{\frac{1}{4}}) \quad \text{--- (*)}
 \end{aligned}$$

Using (**) & (**), we have

$$F_Y(y) = \begin{cases} 0 & \text{if } y < 0 \\ F_X(y^{\frac{1}{4}}) - F_X(-y^{\frac{1}{4}}) & \text{if } 0 \leq y \leq 1 \\ F_X(y^{\frac{1}{4}}) - F_X(-y^{\frac{1}{4}}) & \text{if } 1 < y \leq \frac{81}{16} \\ 1 & \text{if } y > \frac{81}{16} \end{cases}$$

$$= \begin{cases} 0 & \text{if } y < 0 \\ \frac{1}{2} + \frac{1}{3} y^{\frac{1}{4}} - \frac{-y^{\frac{1}{4}} + 1}{2} & \text{if } 0 \leq y \leq 1 \\ \frac{1}{2} + \frac{1}{3} y^{\frac{1}{4}} & \text{if } 1 < y \leq \frac{81}{16} \\ 0 & \text{if } y > \frac{81}{16} \end{cases}$$

$$= \begin{cases} 0 & , \text{ if } y < 0 \\ \frac{5}{6} y^{\frac{1}{4}} & \text{ if } 0 \leq y \leq 1 \\ \frac{1}{2} + \frac{1}{3} y^{\frac{1}{4}} & \text{ if } 1 < y \leq \frac{81}{16} \\ 1 & , \text{ if } y > \frac{81}{16} . \end{cases}$$

~~Wp to this~~

(ii) Hence, the p.d.f. of Y is

$$f_Y(y) = \begin{cases} 0 & \text{if } y < 0 \\ \frac{5}{24} y^{-\frac{3}{4}} & \text{if } 0 \leq y \leq 1 \\ \frac{1}{12} y^{-\frac{3}{4}} & \text{if } 1 < y \leq \frac{81}{16} \\ 0 & \text{if } y > \frac{81}{16} \end{cases}$$

$= \frac{d}{dy} F_Y(y)$